Rotate Function - Update

Rotate Function/rotate_function.dfy
@@ -1,7 +1,7 @@
 method max_rotate_function(nums: array<int>) returns (result: int)
     requires 1 <= nums.Length <= 100000
     requires forall i :: 0 <= i < nums.Length ==> -100 <= nums[i] <= 100
-    ensures forall i :: 0 <= i < nums.Length ==> result >= max_rotate_function_helper(nums, i, 0, nums.Length - 1)
+    ensures max_rotate_function_helper(nums, result, nums.Length)
 {
     var length := nums.Length;
 
@@ -18,7 +18,7 @@ method max_rotate_function(nums: array<int>) returns (result: int)
     var i := 0;
     while (i < length)
         invariant 0 <= i <= length
-        invariant forall k :: 0 <= k < i ==> max >= max_rotate_function_helper(nums, k, 0, length - 1)
+        invariant max_rotate_function_helper(nums, max, i)
     {
         var sum := 0;
         var j := 0;
@@ -39,18 +39,25 @@ method max_rotate_function(nums: array<int>) returns (result: int)
 }
 
 
+predicate max_rotate_function_helper(nums: array<int>, max: int, limit: int)
+    requires 0 <= limit <= nums.Length
+    reads nums
+{
+    forall i :: 0 <= i < limit ==> max >= calculate_rotate_number(nums, i, 0, nums.Length - 1)
+}
+
 function method find_max(x: int, y: int): int
 {
     if x > y then x
     else y
 }
 
-function max_rotate_function_helper(nums: array<int>, position: int, start: int, end: int): int
+function calculate_rotate_number(nums: array<int>, position: int, start: int, end: int): int
     requires 0 <= start <= nums.Length
     requires 0 <= end < nums.Length
     reads nums
     decreases end - start
 {
     if (start > end) then 0
-    else nums[position % nums.Length] * start + max_rotate_function_helper(nums, position + 1, start + 1, end)
+    else nums[position % nums.Length] * start + calculate_rotate_number(nums, position + 1, start + 1, end)
 }
